Learned to stop worrying and love typeclasses (#13)
* Learned to stop worrying and love typeclasses

* And a comment for my own sanity in `term`

* Clean up imports

theories/Context.v
@@ -1,5 +1,6 @@
 From QuickChick Require Import QuickChick.
 From LambdaST Require Import
+  FV
   Terms
   Types.
 From Coq Require Import
@@ -16,9 +17,11 @@ Hint Constructors context : core.
 Derive Show for context.
 Derive Arbitrary for context.
 
-Fixpoint vars_in ctx : list string :=
+Fixpoint fv_ctx ctx : list string :=
   match ctx with
   | CtxEmpty => nil
   | CtxHasTy x _ => cons x nil
-  | CtxComma lhs rhs | CtxSemic lhs rhs => vars_in lhs ++ vars_in rhs
+  | CtxComma lhs rhs | CtxSemic lhs rhs => fv_ctx lhs ++ fv_ctx rhs
   end.
+
+Instance fv_context : FV context := { fv := fv_ctx; }.
