theories/Eqb.v
@@ -1,0 +1,12 @@
+From Coq Require Import
+  Bool
+  String.
+
+Class Eqb (T : Type) := {
+  eqb : T -> T -> bool;
+  eq_dec : forall a b : T, {a = b} + {a <> b};
+  eqb_spec : forall a b : T, reflect (a = b) (eqb a b);
+}.
+
+Instance eqb_string : Eqb string := { eqb := String.eqb; eq_dec := string_dec; eqb_spec := String.eqb_spec; }.
+Instance eqb_bool : Eqb bool := { eqb := Bool.eqb; eq_dec := bool_dec; eqb_spec := Bool.eqb_spec; }.
