theories/FV.v
@@ -1,0 +1,5 @@
+From Coq Require Import
+  List
+  String.
+
+Class FV (T : Type) := { fv : T -> list (* TODO: set *) string }.
